ulib/FStar.MG2.fsti
@@ -1,1 +1,0 @@
-module FSTar.MG2
